for larger examples

src/command.ml
@@ -16,7 +16,8 @@ open Fsm
 
 let default_params : Params.log = Params.Default.log ~mode:(Coq ()) ()
 
-(** [default_bound] is the total depth that will be explored of a given lts by [explore_lts]. *)
+(** [default_bound] is the total depth that will be explored of a given lts by [explore_lts].
+*)
 let default_bound : int = 10
 
 (** [arity_is_prop mip] raises an error if [mip.mind_arity] is not a [prop]. *)
@@ -33,10 +34,11 @@ let arity_is_prop (mip : Declarations.one_inductive_body) : unit mm =
 (** [get_lts_labels_and_terms mib mip] is the mapping of terms (states) and labels (outgoing edges) from [mip].
 
     @raise invalid_arity
-      if lts terms and labels cannot be obtained from [mip]. [mib] is only used in case of error. *)
+      if lts terms and labels cannot be obtained from [mip]. [mib] is only used in case of error.
+*)
 let get_lts_labels_and_terms
-  (mib : Declarations.mutual_inductive_body)
-  (mip : Declarations.one_inductive_body)
+      (mib : Declarations.mutual_inductive_body)
+      (mip : Declarations.one_inductive_body)
   : (Constr.rel_declaration * Constr.rel_declaration) mm
   =
   let open Declarations in
@@ -138,9 +140,9 @@ let check_ref_lts (index : int) (gref : Names.GlobRef.t) : raw_lts mm =
     - Is [w_unify] the best way?
     - ... *)
 let m_unify
-  ?(params : Params.log = default_params)
-  (t0 : EConstr.t)
-  (t1 : EConstr.t)
+      ?(params : Params.log = default_params)
+      (t0 : EConstr.t)
+      (t1 : EConstr.t)
   : bool mm
   =
   params.kind <- Debug ();
@@ -200,8 +202,8 @@ let _pstr_unif_problem (t : unif_problem) : string =
 ;;
 
 let rec unify_all
-  ?(params : Params.log = default_params)
-  (i : (Constr_tree.t * unif_problem) list)
+          ?(params : Params.log = default_params)
+          (i : (Constr_tree.t * unif_problem) list)
   : Constr_tree.t list option mm
   =
   params.kind <- Debug ();
@@ -223,9 +225,9 @@ let rec unify_all
 ;;
 
 let sandboxed_unify
-  ?(params : Params.log = default_params)
-  (tgt_term : EConstr.t)
-  (u : (Constr_tree.t * unif_problem) list)
+      ?(params : Params.log = default_params)
+      (tgt_term : EConstr.t)
+      (u : (Constr_tree.t * unif_problem) list)
   : (EConstr.t * Constr_tree.t list) option mm
   =
   (* let* _ = if is_output_kind_enabled params then debug (fun env sigma -> str
@@ -249,11 +251,11 @@ type coq_ctor = EConstr.t * EConstr.t * Constr_tree.t
 
 (* [act] should probably come from the unification problems? *)
 let rec retrieve_tgt_nodes
-  ?(params : Params.log = default_params)
-  (acc : coq_ctor list)
-  (i : int)
-  (act : EConstr.t)
-  (tgt_term : EConstr.t)
+          ?(params : Params.log = default_params)
+          (acc : coq_ctor list)
+          (i : int)
+          (act : EConstr.t)
+          (tgt_term : EConstr.t)
   : int * (Constr_tree.t * unif_problem) list list -> coq_ctor list mm
   = function
   | _, [] -> return acc
@@ -274,9 +276,9 @@ let rec retrieve_tgt_nodes
 
 (* Should return a list of unification problems *)
 let rec check_updated_ctx
-  ?(params : Params.log = default_params)
-  (acc : int * (Constr_tree.t * unif_problem) list list)
-  (fn_rlts : raw_lts F.t)
+          ?(params : Params.log = default_params)
+          (acc : int * (Constr_tree.t * unif_problem) list list)
+          (fn_rlts : raw_lts F.t)
   :  EConstr.t list * EConstr.rel_declaration list
   -> (int * (Constr_tree.t * unif_problem) list list) option mm
   = function
@@ -338,12 +340,12 @@ let rec check_updated_ctx
 
 (** Checks possible transitions for this term: *)
 and check_valid_constructor
-  ?(params : Params.log = default_params)
-  (ctor_transitions : (Constr.rel_context * Constr.types) array)
-  (fn_rlts : raw_lts F.t)
-  (t' : EConstr.t)
-  (ma : EConstr.t option)
-  (lts_index : int)
+      ?(params : Params.log = default_params)
+      (ctor_transitions : (Constr.rel_context * Constr.types) array)
+      (fn_rlts : raw_lts F.t)
+      (t' : EConstr.t)
+      (ma : EConstr.t option)
+      (lts_index : int)
   : coq_ctor list mm
   =
   params.kind <- Debug ();
@@ -484,7 +486,8 @@ module MkGraph
      and the corresponding [Constr_tree.t]. *)
   module D = P
 
-  (** [constr_transitions] is a hashtbl mapping [action]s to terms of [EConstr.t] and [Constr_tree.t]. *)
+  (** [constr_transitions] is a hashtbl mapping [action]s to terms of [EConstr.t] and [Constr_tree.t].
+  *)
   type constr_transitions = (Mebi_action.action, D.t) Hashtbl.t
 
   let num_transitions (ts : constr_transitions H.t) : int =
@@ -506,18 +509,18 @@ module MkGraph
       List.of_seq (H.to_seq ts)
     in
     let from_body
-      (i : int)
-      (new_transitions :
-        (S.elt * Mebi_action.action * S.elt * Constr_tree.t) list)
+          (i : int)
+          (new_transitions :
+            (S.elt * Mebi_action.action * S.elt * Constr_tree.t) list)
       =
       let (from, actions) : E.t * constr_transitions = List.nth raw_list i in
       let raw_actions : (Mebi_action.action * D.t) list =
         List.of_seq (Hashtbl.to_seq actions)
       in
       let action_body
-        (j : int)
-        (new_transitions :
-          (S.elt * Mebi_action.action * S.elt * Constr_tree.t) list)
+            (j : int)
+            (new_transitions :
+              (S.elt * Mebi_action.action * S.elt * Constr_tree.t) list)
         =
         let (a, destinations) : Mebi_action.action * D.t =
           List.nth raw_actions j
@@ -526,9 +529,9 @@ module MkGraph
           D.elements destinations
         in
         let destination_body
-          (k : int)
-          (new_transitions :
-            (S.elt * Mebi_action.action * S.elt * Constr_tree.t) list)
+              (k : int)
+              (new_transitions :
+                (S.elt * Mebi_action.action * S.elt * Constr_tree.t) list)
           =
           let (destination, constr_tree) : E.t * Constr_tree.t =
             List.nth raw_destinations k
@@ -548,7 +551,8 @@ module MkGraph
     iterate 0 (List.length raw_list - 1) [] from_body
   ;;
 
-  (** [lts_graph] is a record containing a queue of [EConstr.t]s [to_visit], a set of states visited (i.e., [EConstr.t]s), and a hashtbl mapping [EConstr.t] to a map of [constr_transitions], which maps [action]s to [EConstr.t]s and their [Constr_tree.t]. *)
+  (** [lts_graph] is a record containing a queue of [EConstr.t]s [to_visit], a set of states visited (i.e., [EConstr.t]s), and a hashtbl mapping [EConstr.t] to a map of [constr_transitions], which maps [action]s to [EConstr.t]s and their [Constr_tree.t].
+  *)
   type lts_graph =
     { to_visit : E.t Queue.t
     ; init : E.t
@@ -578,8 +582,8 @@ module MkGraph
   ;;
 
   let _print_finished_build_graph
-    ?(params : Params.log = default_params)
-    (g : lts_graph)
+        ?(params : Params.log = default_params)
+        (g : lts_graph)
     : unit mm
     =
     Log.override
@@ -711,12 +715,13 @@ module MkGraph
   (******** above is a sanity check *************************************)
   (**********************************************************************)
 
-  (** [insert_constr_transition] handles adding the mapping of action [a] to tuple [(term * Constr_tree.t)] in a given [constr_transitions]. *)
+  (** [insert_constr_transition] handles adding the mapping of action [a] to tuple [(term * Constr_tree.t)] in a given [constr_transitions].
+  *)
   let insert_constr_transition
-    (constrs : constr_transitions)
-    (a : Mebi_action.action)
-    (d : E.t)
-    (c : Constr_tree.t)
+        (constrs : constr_transitions)
+        (a : Mebi_action.action)
+        (d : E.t)
+        (c : Constr_tree.t)
     : unit mm
     =
     (match Hashtbl.find_opt constrs a with
@@ -726,11 +731,11 @@ module MkGraph
   ;;
 
   let add_new_term_constr_transition
-    (g : lts_graph)
-    (t : E.t)
-    (a : Mebi_action.action)
-    (d : E.t)
-    (c : Constr_tree.t)
+        (g : lts_graph)
+        (t : E.t)
+        (a : Mebi_action.action)
+        (d : E.t)
+        (c : Constr_tree.t)
     : unit mm
     =
     H.add
@@ -741,10 +746,10 @@ module MkGraph
   ;;
 
   let get_new_states
-    ?(params : Params.log = default_params)
-    (t : E.t)
-    (g : lts_graph)
-    (ctors : coq_ctor list)
+        ?(params : Params.log = default_params)
+        (t : E.t)
+        (g : lts_graph)
+        (ctors : coq_ctor list)
     : S.t mm
     =
     let iter_body (i : int) (new_states : S.t) =
@@ -762,9 +767,10 @@ module MkGraph
           insert_constr_transition actions to_add encoding int_tree
       in
       (* if [tgt] has not been explored then add [to_visit] *)
-      if H.mem g.transitions encoding
-         (* || EConstr.eq_constr sigma tgt t *)
-         || S.mem encoding g.states
+      if
+        H.mem g.transitions encoding
+        (* || EConstr.eq_constr sigma tgt t *)
+        || S.mem encoding g.states
       then ()
       else Queue.push encoding g.to_visit;
       (* add [tgt] to [new_states] *)
@@ -776,12 +782,13 @@ module MkGraph
   (** [get_new_constrs t rlts_map] returns the list of constructors applicable to term [t], using those provided in [rlts_map].
       If no immediate constructor is found matching [t] in [rlts_map] (likely due to unification problems), then each constructor in [rlts_map] is tried sequentially, until one of them returns some valid constructors.
       @raise CannotFindTypeOfTermToVisit
-        if none of the constructors provided in [rlts_map] yield constructors from [check_valid_constructors]. *)
+        if none of the constructors provided in [rlts_map] yield constructors from [check_valid_constructors].
+  *)
   let get_new_constrs
-    ?(params : Params.log = default_params)
-    (encoded_t : E.t)
-    (primary : raw_lts)
-    (rlts_map : raw_lts B.t)
+        ?(params : Params.log = default_params)
+        (encoded_t : E.t)
+        (primary : raw_lts)
+        (rlts_map : raw_lts B.t)
     : coq_ctor list mm
     =
     let* (t : EConstr.t) = decode encoded_t in
@@ -801,11 +808,11 @@ module MkGraph
       @param bound is the number of states to explore until.
       @return an [lts_graph] with a maximum of [bound] many states. *)
   let rec build_lts_graph
-    ?(params : Params.log = default_params)
-    (primary : raw_lts)
-    (rlts_map : raw_lts B.t)
-    (g : lts_graph)
-    (bound : int)
+            ?(params : Params.log = default_params)
+            (primary : raw_lts)
+            (rlts_map : raw_lts B.t)
+            (g : lts_graph)
+            (bound : int)
     : lts_graph mm
     =
     params.kind <- Debug ();
@@ -828,7 +835,8 @@ module MkGraph
   ;;
 
   (** @return
-        the key for the primary lts and hashtable mapping the name of the coq definition to the rlts. *)
+        the key for the primary lts and hashtable mapping the name of the coq definition to the rlts.
+  *)
   let build_rlts_map (t' : EConstr.t) (grefs : Names.GlobRef.t list)
     : (E.t * raw_lts B.t) mm
     =
@@ -877,10 +885,10 @@ module MkGraph
       @param tref is the original coq-term.
       @param bound is the number of states to explore until. *)
   let build_graph
-    ?(params : Params.log = default_params)
-    (tref : Constrexpr.constr_expr)
-    (grefs : Names.GlobRef.t list)
-    (bound : int)
+        ?(params : Params.log = default_params)
+        (tref : Constrexpr.constr_expr)
+        (grefs : Names.GlobRef.t list)
+        (bound : int)
     : lts_graph mm
     =
     (* should be able to get the type now -- fail otherwise *)
@@ -918,15 +926,15 @@ module MkGraph
       }
 
     let create_translation_tbl
-      ?(params : Params.log = default_params)
-      (states : S.t)
+          ?(params : Params.log = default_params)
+          (states : S.t)
       : coq_translation mm
       =
       let list_states : E.t list = S.elements states in
       let iter_body
-        (i : int)
-        ((from_coq_list, to_coq_list) :
-          (E.t * string) list * (string * E.t) list)
+            (i : int)
+            ((from_coq_list, to_coq_list) :
+              (E.t * string) list * (string * E.t) list)
         =
         let s : E.t = List.nth list_states i in
         (* let (str : string) = econstr_to_string s in *)
@@ -946,8 +954,8 @@ module MkGraph
     ;;
 
     let _check_all_states_translated
-      (translation_tbl : coq_translation)
-      (g : lts_graph)
+          (translation_tbl : coq_translation)
+          (g : lts_graph)
       : unit mm
       =
       S.iter
@@ -967,10 +975,10 @@ module MkGraph
     ;;
 
     let get_state_translation
-      ?(prefix : string = "?")
-      (state : E.t)
-      (translation_tbl : coq_translation)
-      (g : lts_graph)
+          ?(prefix : string = "?")
+          (state : E.t)
+          (translation_tbl : coq_translation)
+          (g : lts_graph)
       : string mm
       =
       (* let (_str : string) = econstr_to_string state in *)
@@ -1013,10 +1021,10 @@ module MkGraph
     ;;
 
     let translate_transitions
-      (transitions_list :
-        (S.elt * Mebi_action.action * S.elt * Constr_tree.t) list)
-      (translation_tbl : coq_translation)
-      (g : lts_graph)
+          (transitions_list :
+            (S.elt * Mebi_action.action * S.elt * Constr_tree.t) list)
+          (translation_tbl : coq_translation)
+          (g : lts_graph)
       : Lts.raw_flat_lts mm
       =
       (* sanity check: all states should be translated *)
@@ -1065,10 +1073,10 @@ module MkGraph
     ;;
 
     let lts_graph_to_lts
-      ?(params : Params.log = default_params)
-      ?(bound : int = default_bound)
-      ?(name : string = "unnamed")
-      (g : lts_graph)
+          ?(params : Params.log = default_params)
+          ?(bound : int = default_bound)
+          ?(name : string = "unnamed")
+          (g : lts_graph)
       : (Lts.lts * coq_translation) mm
       =
       let* (transitions_list :
@@ -1117,9 +1125,9 @@ let make_graph_builder =
 ;;
 
 let _print_incomplete_lts_warning
-  ?(params : Params.log = default_params)
-  (name : string)
-  (bound : int)
+      ?(params : Params.log = default_params)
+      (name : string)
+      (bound : int)
   : unit
   =
   Log.warning
@@ -1131,8 +1139,8 @@ let _print_incomplete_lts_warning
 ;;
 
 let _print_complete_lts_notice
-  ?(params : Params.log = default_params)
-  (name : string)
+      ?(params : Params.log = default_params)
+      (name : string)
   : unit
   =
   Log.override
@@ -1142,12 +1150,12 @@ let _print_complete_lts_notice
 
 (** *)
 let build_bounded_lts
-  ?(params : Params.log = default_params)
-  ?(bound : int = default_bound)
-  ?(name : string = "unnamed")
-  (tref : Constrexpr.constr_expr)
-  (grefs : Names.GlobRef.t list)
-  (module G : GraphB)
+      ?(params : Params.log = default_params)
+      ?(bound : int = default_bound)
+      ?(name : string = "unnamed")
+      (tref : Constrexpr.constr_expr)
+      (grefs : Names.GlobRef.t list)
+      (module G : GraphB)
   : Lts.lts mm
   =
   Log.override ~params (Printf.sprintf "=-=-=-=-= (building lts of: %s)" name);
@@ -1167,11 +1175,11 @@ let build_bounded_lts
 
 (** *)
 let build_fsm_from_bounded_lts
-  ?(params : Params.log = default_params)
-  ?(bound : int = default_bound)
-  ?(name : string = "unnamed")
-  (tref : Constrexpr.constr_expr)
-  (grefs : Names.GlobRef.t list)
+      ?(params : Params.log = default_params)
+      ?(bound : int = default_bound)
+      ?(name : string = "unnamed")
+      (tref : Constrexpr.constr_expr)
+      (grefs : Names.GlobRef.t list)
   : Fsm.fsm mm
   =
   (* disable detailed printouts *)
@@ -1191,12 +1199,12 @@ let build_fsm_from_bounded_lts
 module Vernac = struct
   module LTS = struct
     let build
-      ?(params : Params.log = default_params)
-      ?(bound : int = default_bound)
-      ?(name : string = "unnamed")
-      ?(equiv : Names.GlobRef.t option)
-      (tref : Constrexpr.constr_expr)
-      (grefs : Names.GlobRef.t list)
+          ?(params : Params.log = default_params)
+          ?(bound : int = default_bound)
+          ?(name : string = "unnamed")
+          ?(equiv : Names.GlobRef.t option)
+          (tref : Constrexpr.constr_expr)
+          (grefs : Names.GlobRef.t list)
       : Lts.lts mm
       =
       (* graph module *)
@@ -1207,11 +1215,11 @@ module Vernac = struct
     ;;
 
     let show
-      ?(params : Params.log = default_params)
-      ?(bound : int = default_bound)
-      ?(equiv : Names.GlobRef.t option)
-      (tref : Constrexpr.constr_expr)
-      (grefs : Names.GlobRef.t list)
+          ?(params : Params.log = default_params)
+          ?(bound : int = default_bound)
+          ?(equiv : Names.GlobRef.t option)
+          (tref : Constrexpr.constr_expr)
+          (grefs : Names.GlobRef.t list)
       : unit mm
       =
       let* (the_lts : Lts.lts) = build ~params ~bound tref grefs in
@@ -1222,16 +1230,17 @@ module Vernac = struct
     ;;
 
     let dump
-      ?(params : Params.log = default_params)
-      ?(bound : int = default_bound)
-      ?(name : string = "dump")
-      ?(equiv : Names.GlobRef.t option)
-      (tref : Constrexpr.constr_expr)
-      (grefs : Names.GlobRef.t list)
+          ?(params : Params.log = default_params)
+          ?(bound : int = default_bound)
+          ?(name : string = "dump")
+          ?(equiv : Names.GlobRef.t option)
+          (tref : Constrexpr.constr_expr)
+          (grefs : Names.GlobRef.t list)
       : unit mm
       =
       params.options.output_enabled <- false;
       let* (the_lts : Lts.lts) = build ~params ~bound ~name tref grefs in
+      Log.override ~params (Printf.sprintf "- - - - (dumping lts of: %s)" name);
       let dump_filepath : string =
         Dump_to_file.write_to_file
           (Default ())
@@ -1247,23 +1256,23 @@ module Vernac = struct
   module FSM = struct
     (** *)
     let build
-      ?(params : Params.log = default_params)
-      ?(bound : int = default_bound)
-      ?(name : string = "unnamed")
-      ?(equiv : Names.GlobRef.t option)
-      (tref : Constrexpr.constr_expr)
-      (grefs : Names.GlobRef.t list)
+          ?(params : Params.log = default_params)
+          ?(bound : int = default_bound)
+          ?(name : string = "unnamed")
+          ?(equiv : Names.GlobRef.t option)
+          (tref : Constrexpr.constr_expr)
+          (grefs : Names.GlobRef.t list)
       : Fsm.fsm mm
       =
       build_fsm_from_bounded_lts ~params ~bound ~name tref grefs
     ;;
 
     let show
-      ?(params : Params.log = default_params)
-      ?(bound : int = default_bound)
-      ?(equiv : Names.GlobRef.t option)
-      (tref : Constrexpr.constr_expr)
-      (grefs : Names.GlobRef.t list)
+          ?(params : Params.log = default_params)
+          ?(bound : int = default_bound)
+          ?(equiv : Names.GlobRef.t option)
+          (tref : Constrexpr.constr_expr)
+          (grefs : Names.GlobRef.t list)
       : unit mm
       =
       (* get translated fsm *)
@@ -1279,24 +1288,26 @@ module Vernac = struct
     ;;
 
     let dump
-      ?(params : Params.log = default_params)
-      ?(bound : int = default_bound)
-      ?(name : string = "dump")
-      ?(equiv : Names.GlobRef.t option)
-      (tref : Constrexpr.constr_expr)
-      (grefs : Names.GlobRef.t list)
+          ?(params : Params.log = default_params)
+          ?(bound : int = default_bound)
+          ?(name : string = "dump")
+          ?(equiv : Names.GlobRef.t option)
+          (tref : Constrexpr.constr_expr)
+          (grefs : Names.GlobRef.t list)
       : unit mm
       =
       (* get translated fsm *)
       let* the_fsm = build ~params ~bound ~name tref grefs in
-      let dump_filepath : string =
-        Dump_to_file.write_to_file
-          (Default ())
-          (FSM name)
-          (JSON ())
-          (FSM the_fsm)
-      in
-      log ~params (Printf.sprintf "Dumped FSM into: %s.\n" dump_filepath);
+      Log.override ~params (Printf.sprintf "TODO: (dumping fsm of: %s)" name);
+      (* Log.override ~params (Printf.sprintf "- - - - (dumping fsm of: %s)" name);
+         let dump_filepath : string =
+         Dump_to_file.write_to_file
+         (Default ())
+         (FSM name)
+         (JSON ())
+         (FSM the_fsm)
+         in
+         log ~params (Printf.sprintf "Dumped FSM into: %s.\n" dump_filepath); *)
       return ()
     ;;
   end
@@ -1304,11 +1315,11 @@ module Vernac = struct
   module Minim = struct
     (** *)
     let build
-      ?(params : Params.log = default_params)
-      ?(bound : int = default_bound)
-      ?(name : string = "unnamed")
-      (tref : Constrexpr.constr_expr)
-      (grefs : Names.GlobRef.t list)
+          ?(params : Params.log = default_params)
+          ?(bound : int = default_bound)
+          ?(name : string = "unnamed")
+          (tref : Constrexpr.constr_expr)
+          (grefs : Names.GlobRef.t list)
       : (Fsm.fsm * Fsm.fsm) mm
       =
       (* get translated fsm *)
@@ -1321,10 +1332,10 @@ module Vernac = struct
 
     (** *)
     let show
-      ?(params : Params.log = default_params)
-      ?(bound : int = default_bound)
-      (tref : Constrexpr.constr_expr)
-      (grefs : Names.GlobRef.t list)
+          ?(params : Params.log = default_params)
+          ?(bound : int = default_bound)
+          (tref : Constrexpr.constr_expr)
+          (grefs : Names.GlobRef.t list)
       : unit mm
       =
       (* get translated fsm *)
@@ -1343,34 +1354,35 @@ module Vernac = struct
     ;;
 
     let dump
-      ?(params : Params.log = default_params)
-      ?(bound : int = default_bound)
-      ?(name : string = "dump")
-      (tref : Constrexpr.constr_expr)
-      (grefs : Names.GlobRef.t list)
+          ?(params : Params.log = default_params)
+          ?(bound : int = default_bound)
+          ?(name : string = "dump")
+          (tref : Constrexpr.constr_expr)
+          (grefs : Names.GlobRef.t list)
       : unit mm
       =
       (* get translated fsm *)
       let* the_fsm, minimized_fsm = build ~params ~bound ~name tref grefs in
-      let fsm_dump_filepath : string =
-        Dump_to_file.write_to_file
-          (Default ())
-          (FSM (Printf.sprintf "%s tobe minim" name))
-          (JSON ())
-          (FSM the_fsm)
-      and minim_dump_filepath : string =
-        Dump_to_file.write_to_file
-          (Default ())
-          (FSM (Printf.sprintf "%s post minim" name))
-          (JSON ())
-          (FSM minimized_fsm)
-      in
-      log
-        ~params
-        (Printf.sprintf
-           "Dumped FSMs into: %s\nand %s.\n"
-           fsm_dump_filepath
-           minim_dump_filepath);
+      Log.override ~params (Printf.sprintf "TODO: (dumping fsm of: %s)" name);
+      (* let fsm_dump_filepath : string =
+         Dump_to_file.write_to_file
+         (Default ())
+         (FSM (Printf.sprintf "%s tobe minim" name))
+         (JSON ())
+         (FSM the_fsm)
+         and minim_dump_filepath : string =
+         Dump_to_file.write_to_file
+         (Default ())
+         (FSM (Printf.sprintf "%s post minim" name))
+         (JSON ())
+         (FSM minimized_fsm)
+         in
+         log
+         ~params
+         (Printf.sprintf
+         "Dumped FSMs into: %s\nand %s.\n"
+         fsm_dump_filepath
+         minim_dump_filepath); *)
       return ()
     ;;
   end
@@ -1378,12 +1390,12 @@ module Vernac = struct
   module Merged = struct
     (** *)
     let build
-      ?(params : Params.log = default_params)
-      ?(bound : int = default_bound)
-      ?(name : string = "unnamed")
-      (trefA : Constrexpr.constr_expr)
-      (trefB : Constrexpr.constr_expr)
-      (grefs : Names.GlobRef.t list)
+          ?(params : Params.log = default_params)
+          ?(bound : int = default_bound)
+          ?(name : string = "unnamed")
+          (trefA : Constrexpr.constr_expr)
+          (trefB : Constrexpr.constr_expr)
+          (grefs : Names.GlobRef.t list)
       : (Fsm.fsm * Fsm.fsm * Fsm.fsm) mm
       =
       (* get translated fsm *)
@@ -1402,11 +1414,11 @@ module Vernac = struct
 
     (** *)
     let show
-      ?(params : Params.log = default_params)
-      ?(bound : int = default_bound)
-      (trefA : Constrexpr.constr_expr)
-      (trefB : Constrexpr.constr_expr)
-      (grefs : Names.GlobRef.t list)
+          ?(params : Params.log = default_params)
+          ?(bound : int = default_bound)
+          (trefA : Constrexpr.constr_expr)
+          (trefB : Constrexpr.constr_expr)
+          (grefs : Names.GlobRef.t list)
       : unit mm
       =
       (* get merged fsm *)
@@ -1426,44 +1438,45 @@ module Vernac = struct
     ;;
 
     let dump
-      ?(params : Params.log = default_params)
-      ?(bound : int = default_bound)
-      ?(name : string = "dump")
-      (trefA : Constrexpr.constr_expr)
-      (trefB : Constrexpr.constr_expr)
-      (grefs : Names.GlobRef.t list)
+          ?(params : Params.log = default_params)
+          ?(bound : int = default_bound)
+          ?(name : string = "dump")
+          (trefA : Constrexpr.constr_expr)
+          (trefB : Constrexpr.constr_expr)
+          (grefs : Names.GlobRef.t list)
       : unit mm
       =
       (* get merged fsm *)
       let* merged_fsm, fsm_A, fsm_B =
         build ~params ~bound ~name trefA trefB grefs
       in
-      let merged_dump_filepath : string =
-        Dump_to_file.write_to_file
-          (Default ())
-          (FSM (Printf.sprintf "%s merged fsm" name))
-          (JSON ())
-          (FSM merged_fsm)
-      and fsm_a_dump_filepath : string =
-        Dump_to_file.write_to_file
-          (Default ())
-          (FSM (Printf.sprintf "%s to merge A" name))
-          (JSON ())
-          (FSM fsm_A)
-      and fsm_b_dump_filepath : string =
-        Dump_to_file.write_to_file
-          (Default ())
-          (FSM (Printf.sprintf "%s to merge B" name))
-          (JSON ())
-          (FSM fsm_B)
-      in
-      log
-        ~params
-        (Printf.sprintf
-           "Dumped FSMs into: %s\nand %s\nand %s.\n"
-           merged_dump_filepath
-           fsm_a_dump_filepath
-           fsm_b_dump_filepath);
+      Log.override ~params (Printf.sprintf "TODO: (dumping fsm of: %s)" name);
+      (* let merged_dump_filepath : string =
+         Dump_to_file.write_to_file
+         (Default ())
+         (FSM (Printf.sprintf "%s merged fsm" name))
+         (JSON ())
+         (FSM merged_fsm)
+         and fsm_a_dump_filepath : string =
+         Dump_to_file.write_to_file
+         (Default ())
+         (FSM (Printf.sprintf "%s to merge A" name))
+         (JSON ())
+         (FSM fsm_A)
+         and fsm_b_dump_filepath : string =
+         Dump_to_file.write_to_file
+         (Default ())
+         (FSM (Printf.sprintf "%s to merge B" name))
+         (JSON ())
+         (FSM fsm_B)
+         in
+         log
+         ~params
+         (Printf.sprintf
+         "Dumped FSMs into: %s\nand %s\nand %s.\n"
+         merged_dump_filepath
+         fsm_a_dump_filepath
+         fsm_b_dump_filepath); *)
       return ()
     ;;
   end
@@ -1475,12 +1488,12 @@ module Vernac = struct
 
     (** *)
     let build
-      ?(params : Params.log = default_params)
-      ?(bound : int = default_bound)
-      ?(name : string = "unnamed")
-      (trefA : Constrexpr.constr_expr)
-      (trefB : Constrexpr.constr_expr)
-      (grefs : Names.GlobRef.t list)
+          ?(params : Params.log = default_params)
+          ?(bound : int = default_bound)
+          ?(name : string = "unnamed")
+          (trefA : Constrexpr.constr_expr)
+          (trefB : Constrexpr.constr_expr)
+          (grefs : Names.GlobRef.t list)
       : (Fsm.fsm * Fsm.fsm * Bisimilarity.result) mm
       =
       (* get translated fsm *)
@@ -1498,11 +1511,11 @@ module Vernac = struct
 
     (** *)
     let show
-      ?(params : Params.log = default_params)
-      ?(bound : int = default_bound)
-      (trefA : Constrexpr.constr_expr)
-      (trefB : Constrexpr.constr_expr)
-      (grefs : Names.GlobRef.t list)
+          ?(params : Params.log = default_params)
+          ?(bound : int = default_bound)
+          (trefA : Constrexpr.constr_expr)
+          (trefB : Constrexpr.constr_expr)
+          (grefs : Names.GlobRef.t list)
       : unit mm
       =
       let* fsm_A, fsm_B, result = build ~params ~bound trefA trefB grefs in
@@ -1523,47 +1536,48 @@ module Vernac = struct
     ;;
 
     let dump
-      ?(params : Params.log = default_params)
-      ?(bound : int = default_bound)
-      ?(name : string = "dump")
-      (trefA : Constrexpr.constr_expr)
-      (trefB : Constrexpr.constr_expr)
-      (grefs : Names.GlobRef.t list)
+          ?(params : Params.log = default_params)
+          ?(bound : int = default_bound)
+          ?(name : string = "dump")
+          (trefA : Constrexpr.constr_expr)
+          (trefB : Constrexpr.constr_expr)
+          (grefs : Names.GlobRef.t list)
       : unit mm
       =
       let* fsm_A, fsm_B, result =
         build ~params ~bound ~name trefA trefB grefs
       in
-      match result with
-      | BisimResult result ->
-        let merged_dump_filepath : string =
-          Dump_to_file.write_to_file
-            (Default ())
-            (FSM (Printf.sprintf "%s bisim merged fsm" name))
-            (JSON ())
-            (FSM result.merged_fsm)
-        and fsm_a_dump_filepath : string =
-          Dump_to_file.write_to_file
-            (Default ())
-            (FSM (Printf.sprintf "%s bisim to merge A" name))
-            (JSON ())
-            (FSM fsm_A)
-        and fsm_b_dump_filepath : string =
-          Dump_to_file.write_to_file
-            (Default ())
-            (FSM (Printf.sprintf "%s bisim to merge B" name))
-            (JSON ())
-            (FSM fsm_B)
-        in
-        log
-          ~params
-          (Printf.sprintf
-             "Dumped FSMs into: %s\nand %s\nand %s.\n"
-             merged_dump_filepath
-             fsm_a_dump_filepath
-             fsm_b_dump_filepath);
-        return ()
-      | _ -> raise (UnexpectedResultKind result)
+      Log.override ~params (Printf.sprintf "TODO: (dumping fsm of: %s)" name);
+      (* (match result with
+         | BisimResult result ->
+         let merged_dump_filepath : string =
+         Dump_to_file.write_to_file
+         (Default ())
+         (FSM (Printf.sprintf "%s bisim merged fsm" name))
+         (JSON ())
+         (FSM result.merged_fsm)
+         and fsm_a_dump_filepath : string =
+         Dump_to_file.write_to_file
+         (Default ())
+         (FSM (Printf.sprintf "%s bisim to merge A" name))
+         (JSON ())
+         (FSM fsm_A)
+         and fsm_b_dump_filepath : string =
+         Dump_to_file.write_to_file
+         (Default ())
+         (FSM (Printf.sprintf "%s bisim to merge B" name))
+         (JSON ())
+         (FSM fsm_B)
+         in
+         log
+         ~params
+         (Printf.sprintf
+         "Dumped FSMs into: %s\nand %s\nand %s.\n"
+         merged_dump_filepath
+         fsm_a_dump_filepath
+         fsm_b_dump_filepath);
+         | _ -> raise (UnexpectedResultKind result)); *)
+      return ()
     ;;
   end
 end
@@ -1582,4 +1596,5 @@ end
     Notes:
     - Constructors of [P] are the transitions
     - States are the sets of possible transitions
-    - A term [t] is represented by the state of the transitions that can be taken *)
+    - A term [t] is represented by the state of the transitions that can be taken
+*)
